WellTyped.v
@@ -1,9 +1,133 @@
 Require Import Common.
-Require Import Lang.
 Require Import List.
+Require Import sflib.
 
+Require Import Value.
+Require Import Lang.
+Require Import State.
 
 Module Ir.
+
+Inductive inst_typechecked (md:Ir.IRModule.t) (st:Ir.Config.t)
+:Prop :=
+| tc_bop:
+    forall op1 op2 r opty bopc i1 i2 bsz
+           (HINST: Some (Ir.Inst.ibinop r opty bopc op1 op2) =
+                Ir.Config.cur_inst md st)
+           (HTY: Ir.ity bsz = opty)
+           (HOP1: Some (Ir.num i1) = Ir.Config.get_val st op1)
+           (HOP2: Some (Ir.num i2) = Ir.Config.get_val st op2),
+        inst_typechecked md st
+| tc_psub:
+    forall op1 op2 r retty ptrty p1 p2 bsz pty
+           (HINST: Some (Ir.Inst.ipsub r retty ptrty op1 op2) =
+                Ir.Config.cur_inst md st)
+           (HRETTY: Ir.ity bsz = retty)
+           (HPTY: Ir.ptrty pty = ptrty)
+           (HOP1: Some (Ir.ptr p1) = Ir.Config.get_val st op1)
+           (HOP2: Some (Ir.ptr p2) = Ir.Config.get_val st op1),
+        inst_typechecked md st
+| tc_gep:
+    forall op1 op2 r ptrty p i pty inb
+           (HINST: Some (Ir.Inst.igep r ptrty op1 op2 inb) =
+                Ir.Config.cur_inst md st)
+           (HPTY: Ir.ptrty pty = ptrty)
+           (HOP1: Some (Ir.ptr p) = Ir.Config.get_val st op1)
+           (HOP2: Some (Ir.num i) = Ir.Config.get_val st op2),
+        inst_typechecked md st
+| tc_load:
+    forall retty opval opptr p
+        (HINST: Some (Ir.Inst.iload retty opval opptr) =
+                Ir.Config.cur_inst md st)
+        (HOPPTR: Some (Ir.ptr p) = Ir.Config.get_val st opptr),
+        inst_typechecked md st
+| tc_store:
+    forall valty opval opptr p v
+           (HINST: Some (Ir.Inst.istore valty opptr opval) =
+                Ir.Config.cur_inst md st)
+           (HOPPTR: Some (Ir.ptr p) = Ir.Config.get_val st opptr)
+           (HOPVAL: Some v = Ir.Config.get_val st opval),
+        inst_typechecked md st
+| tc_malloc:
+    forall opty opval i sz r
+           (HINST: Some (Ir.Inst.imalloc r opty opval) =
+                Ir.Config.cur_inst md st)
+           (HOPPTR: Some (Ir.num i) = Ir.Config.get_val st opval)
+           (HSZTY: Ir.ity sz = opty),
+        inst_typechecked md st
+| tc_bitcast_int:
+    forall r opval retty bsz i1
+           (HINST: Some (Ir.Inst.ibitcast r opval retty) =
+                Ir.Config.cur_inst md st)
+           (HTY: Ir.ity bsz = retty)
+           (HOP1: Some (Ir.num i1) = Ir.Config.get_val st opval),
+        inst_typechecked md st
+| tc_bitcast_ptr:
+    forall r opval retty pty p
+           (HINST: Some (Ir.Inst.ibitcast r opval retty) =
+                Ir.Config.cur_inst md st)
+           (HTY: Ir.ptrty pty = retty)
+           (HOP1: Some (Ir.ptr p) = Ir.Config.get_val st opval),
+        inst_typechecked md st
+| tc_ptrtoint:
+    forall r opval retty bsz p
+           (HINST: Some (Ir.Inst.iptrtoint r opval retty) =
+                Ir.Config.cur_inst md st)
+           (HTY: Ir.ity bsz = retty)
+           (HOP1: Some (Ir.ptr p) = Ir.Config.get_val st opval),
+        inst_typechecked md st
+| tc_inttoptr:
+    forall r opval retty pty i
+           (HINST: Some (Ir.Inst.iinttoptr r opval retty) =
+                Ir.Config.cur_inst md st)
+           (HTY: Ir.ptrty pty = retty)
+           (HOP1: Some (Ir.num i) = Ir.Config.get_val st opval),
+        inst_typechecked md st
+| tc_event:
+    forall opval i
+           (HINST: Some (Ir.Inst.ievent opval) =
+                Ir.Config.cur_inst md st)
+           (HOP1: Some (Ir.num i) = Ir.Config.get_val st opval),
+        inst_typechecked md st
+| tc_icmpeq_int:
+    forall op1 op2 r opty i1 i2 bsz
+           (HINST: Some (Ir.Inst.iicmp_eq r opty op1 op2) =
+                Ir.Config.cur_inst md st)
+           (HTY: Ir.ity bsz = opty)
+           (HOP1: Some (Ir.num i1) = Ir.Config.get_val st op1)
+           (HOP2: Some (Ir.num i2) = Ir.Config.get_val st op2),
+        inst_typechecked md st
+| tc_icmpeq_ptr:
+    forall op1 op2 r opty p1 p2 pty
+           (HINST: Some (Ir.Inst.iicmp_eq r opty op1 op2) =
+                Ir.Config.cur_inst md st)
+           (HTY: Ir.ptrty pty = opty)
+           (HOP1: Some (Ir.ptr p1) = Ir.Config.get_val st op1)
+           (HOP2: Some (Ir.ptr p2) = Ir.Config.get_val st op2),
+        inst_typechecked md st
+| tc_icmpule_int:
+    forall op1 op2 r opty i1 i2 bsz
+           (HINST: Some (Ir.Inst.iicmp_ule r opty op1 op2) =
+                Ir.Config.cur_inst md st)
+           (HTY: Ir.ity bsz = opty)
+           (HOP1: Some (Ir.num i1) = Ir.Config.get_val st op1)
+           (HOP2: Some (Ir.num i2) = Ir.Config.get_val st op2),
+        inst_typechecked md st
+| tc_icmpule_ptr:
+    forall op1 op2 r opty p1 p2 pty
+           (HINST: Some (Ir.Inst.iicmp_ule r opty op1 op2) =
+                Ir.Config.cur_inst md st)
+           (HTY: Ir.ptrty pty = opty)
+           (HOP1: Some (Ir.ptr p1) = Ir.Config.get_val st op1)
+           (HOP2: Some (Ir.ptr p2) = Ir.Config.get_val st op2),
+        inst_typechecked md st
+| tc_free:
+    forall opptr p
+        (HINST: Some (Ir.Inst.ifree opptr) =
+                Ir.Config.cur_inst md st)
+        (HOPPTR: Some (Ir.ptr p) = Ir.Config.get_val st opptr),
+        inst_typechecked md st.
+
 
 (****************************************
         Dominatedness relation.
@@ -47,14 +171,5 @@ Proof.
     apply Gt.gt_Sn_O.
 Qed.
 
-
-Structure welltyped (m:Ir.IRModule.t) :=
-  {
-    ssa:forall (f:Ir.IRFunction.t)
-               (HFIN:List.In f m)
-               (r:Ir.reg),
-      List.length (Ir.IRFunction.get_defs r f) < 2;
-    
-  }.
 
 End Ir.
